Splinter/Betree/FilteredBetreeRefinement.i.dfy
@@ -1,0 +1,700 @@
+// Copyright 2018-2021 VMware, Inc., Microsoft Inc., Carnegie Mellon University, ETH Zurich, and University of Washington
+// SPDX-License-Identifier: BSD-2-Clause
+
+// include "PivotBetree.i.dfy"
+include "FilteredBetree.i.dfy"
+include "PivotBetreeRefinement.i.dfy"
+
+module FilteredBetreeRefinement
+{
+  import opened Options
+  import opened KeyType
+  import opened StampedMod
+  import TotalKMMapMod
+  import opened ValueMessage
+  import opened MsgHistoryMod
+  import opened LSNMod
+  import opened Sequences
+  import opened Buffers
+  import opened MemtableMod
+  import opened Upperbounded_Lexicographic_Byte_Order_Impl
+  import opened Upperbounded_Lexicographic_Byte_Order_Impl.Ord
+  import opened BoundedPivotsLib
+  import opened DomainMod
+  import opened FilteredBetree
+  import PivotBetree
+  import PivotBetreeRefinement
+
+  function ActiveBufferKeysForChild(node: BetreeNode, childIdx: nat, bufferIdx: nat) : iset<Key>
+    requires node.WF()
+    requires node.BetreeNode?
+    requires childIdx < |node.children|
+    requires bufferIdx < node.buffers.Length()
+  {
+    if node.activeBufferRanges[childIdx] <= bufferIdx 
+    then node.DomainRoutedToChild(childIdx).KeySet()
+    else iset{}
+  }
+
+  function ActiveBufferKeys(node: BetreeNode, bufferIdx: nat) : iset<Key>
+    requires node.WF()
+    requires node.BetreeNode?
+    requires bufferIdx < node.buffers.Length()
+  {
+    iset k, i | 0 <= i < |node.children| && k in ActiveBufferKeysForChild(node, i, bufferIdx) :: k
+  }
+
+  function IBuffer(node: BetreeNode, bufferIdx: nat) : Buffer
+    requires node.WF()
+    requires node.BetreeNode?
+    requires bufferIdx < node.buffers.Length()
+  {
+    node.buffers.buffers[bufferIdx].ApplyFilter(ActiveBufferKeys(node, bufferIdx))
+  }
+
+  function IBufferStack(node: BetreeNode) : BufferStack
+    requires node.WF()
+    requires node.BetreeNode?
+  {
+    BufferStack(seq (node.buffers.Length(), i requires 0 <= i < node.buffers.Length() => IBuffer(node, i)))
+  }
+
+  function IChildren(node: BetreeNode) : (out: seq<PivotBetree.BetreeNode>)
+    requires node.WF()
+    requires node.BetreeNode?
+    decreases node, 0
+  {
+    assert WFChildren(node.children); // trigger
+    seq (|node.children|, i requires 0 <= i < |node.children| => INode(node.children[i]))
+  }
+
+  function INode(node: BetreeNode) : (out: PivotBetree.BetreeNode)
+    requires node.WF()
+    ensures out.WF()
+    ensures node.Nil? <==> out.Nil?
+    decreases node, 1
+  {
+    var out := 
+      if node.Nil?
+      then PivotBetree.Nil
+      else PivotBetree.BetreeNode(IBufferStack(node), node.pivotTable, IChildren(node));
+
+    assert out.WF() by {
+      forall i:nat |
+        && out.ValidChildIndex(i)
+        && out.children[i].BetreeNode?
+        && out.children[i].LocalStructure()
+        ensures out.children[i].MyDomain() == out.DomainRoutedToChild(i) {
+          assert WFChildren(node.children); // trigger
+          assert out.children[i] == IChildren(node)[i]; // trigger
+          // assert out.DomainRoutedToChild(i) == node.DomainRoutedToChild(i);  // trigger
+       }
+    }
+    out
+  }
+
+  function IStampedBetree(stampedBetree: StampedBetree) : PivotBetree.StampedBetree
+    requires stampedBetree.value.WF()
+  {
+    Stamped(INode(stampedBetree.value), stampedBetree.seqEnd)
+  }
+
+  function ILbl(lbl: TransitionLabel) : PivotBetree.TransitionLabel
+  {
+    match lbl
+      case QueryLabel(endLsn, key, value) => PivotBetree.QueryLabel(endLsn, key, value)
+      case PutLabel(puts) => PivotBetree.PutLabel(puts)
+      case QueryEndLsnLabel(endLsn) => PivotBetree.QueryEndLsnLabel(endLsn)
+      case FreezeAsLabel(stampedBetree) => PivotBetree.FreezeAsLabel(
+        if stampedBetree.value.WF()
+        then IStampedBetree(stampedBetree)
+        else PivotBetree.EmptyImage())
+      case InternalLabel() => PivotBetree.InternalLabel()
+  }
+
+  function I(v: Variables) : PivotBetree.Variables
+    requires v.WF()
+  {
+    PivotBetree.Variables(v.memtable, INode(v.root))
+  }
+
+  predicate Inv(v: Variables)
+  {
+    && v.WF()
+    && (v.root.BetreeNode? ==> v.root.MyDomain() == TotalDomain())
+  }
+
+  // lemma InvNext(v: Variables, v': Variables, lbl: TransitionLabel)
+  //   requires Inv(v)
+  //   requires Next(v, v', lbl)
+  //   ensures Inv(v')
+  // {
+  //   if v'.root.BetreeNode? {
+  //     var step :| NextStep(v, v', lbl, step);
+  //     if step.InternalSplitStep? {
+  //       SubstitutePreservesWF(step.path, step.path.Target().SplitParent(step.request));
+  //     } else if step.InternalFlushStep? {
+  //       SubstitutePreservesWF(step.path, step.path.Target().Flush(step.childIdx));
+  //     } else if step.InternalCompactStep? {
+  //       var compactedNode := CompactedNode(step.path.Target(), step.compactedBuffers);
+  //       SubstitutePreservesWF(step.path, compactedNode);
+  //     }
+  //   }
+  //   assert v'.root.WF();  // trigger
+  // }
+
+  function IPath(path: Path) : (out: PivotBetree.Path)
+    requires path.Valid()
+  {
+    PivotBetree.Path(INode(path.node), path.key, path.depth)
+  }
+
+  lemma SubpathCommutesWithIPath(path: Path) 
+    requires path.Valid()
+    requires 0 < path.depth
+    ensures IPath(path.Subpath()) == IPath(path).Subpath()
+  {
+    calc {  // trigger
+        IPath(Path(path.node.Child(path.key), path.key, path.depth-1));
+        PivotBetree.Path(INode(path.node), path.key, path.depth).Subpath();
+      }
+  }
+
+  lemma IPathValid(path: Path) 
+    requires path.Valid()
+    ensures IPath(path).Valid()
+    decreases path.depth
+  {
+    if 0 < path.depth {
+      SubpathCommutesWithIPath(path);
+      IPathValid(path.Subpath());
+      assert IPath(path).node == INode(path.node); // trigger
+    }
+  }
+
+  function IReceiptLine(line: QueryReceiptLine) : PivotBetree.QueryReceiptLine
+    requires line.WF()
+  {
+    PivotBetree.QueryReceiptLine(INode(line.node), line.result)
+  }
+
+  function IReceipt(receipt: QueryReceipt) : PivotBetree.QueryReceipt
+    requires receipt.Valid()
+  {
+    PivotBetree.QueryReceipt(receipt.key, INode(receipt.root),
+      seq(|receipt.lines|, i requires 0<=i<|receipt.lines| => IReceiptLine(receipt.lines[i])))
+  }
+
+  lemma IReceiptValid(receipt: QueryReceipt) 
+    requires receipt.Valid()
+    ensures IReceipt(receipt).Valid()
+  {
+    var ireceipt := IReceipt(receipt);
+    var key := receipt.key;
+
+    forall i:nat | i < |ireceipt.lines|-1 
+      ensures ireceipt.lines[i].node.KeyInDomain(key)
+      ensures ireceipt.ChildLinkedAt(i)
+    {
+      assert receipt.lines[i].node.KeyInDomain(key);  // trigger
+      assert receipt.ChildLinkedAt(i);  // trigger
+      ChildKeyCommutesWithI(receipt.lines[i].node, key);
+    }
+  
+    forall i:nat | i < |ireceipt.lines| - 1 
+    ensures ireceipt.ResultLinkedAt(i)
+    {
+      assert receipt.ResultLinkedAt(i);  // trigger
+      var node := receipt.lines[i].node;
+      var key := ireceipt.key;
+      QueryCommutesWithIBufferStack(node, key, node.ActiveBuffersForKey(key), node.buffers.Length());
+    }
+  }
+
+  lemma ChildKeyCommutesWithI(node: BetreeNode, key: Key)
+    requires node.WF()
+    requires node.KeyInDomain(key)
+    ensures node.Child(key).WF()
+    ensures INode(node.Child(key)) == INode(node).Child(key)
+  {
+  }
+
+  lemma ActiveBuffersForKeyConsistent(node: BetreeNode, key: Key, start: nat)
+    requires node.WF()
+    requires node.KeyInDomain(key)
+    requires start == node.ActiveBuffersForKey(key)
+    ensures forall i:nat | i < start :: key !in ActiveBufferKeys(node, i)
+    ensures forall i:nat | start <= i < node.buffers.Length() :: key in ActiveBufferKeys(node, i)
+  {
+    forall i:nat | start <= i < node.buffers.Length()
+      ensures key in ActiveBufferKeys(node, i)
+    {
+      var childIdx := Route(node.pivotTable, key);
+      assert key in ActiveBufferKeysForChild(node, childIdx, i); // trigger
+    }
+  }
+
+  lemma QueryCommutesWithIBufferStack(node: BetreeNode, key: Key, start: nat, count: nat)
+    requires IBufferStack.requires(node)
+    requires node.KeyInDomain(key)
+    requires count <= node.buffers.Length()
+    requires start == node.ActiveBuffersForKey(key)
+    ensures count <= start ==> (IBufferStack(node).QueryUpTo(key, count) == Update(NopDelta()))
+    ensures start < count ==> (IBufferStack(node).QueryUpTo(key, count) == 
+      node.buffers.Slice(start, node.buffers.Length()).QueryUpTo(key, count-start))
+  {
+    ActiveBuffersForKeyConsistent(node, key, start);
+    if start < count || 0 < count {
+      QueryCommutesWithIBufferStack(node, key, start, count-1);
+    }
+  }
+
+  function IStepDefn(step: Step) : (out: PivotBetree.Step)
+    requires step.WF()
+  {
+    match step {
+      case QueryStep(receipt) => PivotBetree.QueryStep(IReceipt(receipt))
+      case PutStep() => PivotBetree.PutStep()
+      case QueryEndLsnStep() => PivotBetree.QueryEndLsnStep()
+      case FreezeAsStep() => PivotBetree.FreezeAsStep()
+      case InternalGrowStep() => PivotBetree.InternalGrowStep()
+      case  InternalSplitStep(path, request) => PivotBetree.InternalSplitStep(IPath(path), request)
+      case InternalFlushStep(path, childIdx, _) => PivotBetree.InternalFlushStep(IPath(path), childIdx)
+      case InternalFlushMemtableStep() => PivotBetree.InternalFlushMemtableStep()
+      case InternalCompactStep(path, compactStart, compactEnd, compactedBuffer) => (
+        var buffers := IBufferStack(path.Target()).buffers;
+        var compactedBuffers := BufferStack(buffers[..compactStart] + [compactedBuffer] + buffers[compactEnd..]);
+        PivotBetree.InternalCompactStep(IPath(path), compactedBuffers)
+      )
+      case InternalNoOpStep() => PivotBetree.InternalNoOpStep()
+    }
+  }
+
+  lemma IStepWF(step: Step)
+    requires IStepDefn.requires(step)
+    ensures IStepDefn(step).WF()
+  {
+    var istep := IStepDefn(step);
+    match step {
+      case QueryStep(receipt) => { IReceiptValid(receipt); }
+      case InternalSplitStep(path, request) => { assume false; }//TargetCommutesWithI(path); }
+      case InternalFlushStep(path, childIdx, _) => { assume false; }//TargetCommutesWithI(path); }
+      case InternalCompactStep(path, compactStart, compactEnd, compactedBuffer) => { assume false; }//InternalCompactStepWF(step); }
+      case _ => { assert istep.WF(); }
+    }
+  }
+
+  function IStep(step: Step) : (out: PivotBetree.Step)
+    requires step.WF()
+    ensures out.WF()
+  {
+    IStepWF(step);
+    IStepDefn(step)
+  }
+
+  lemma InitRefines(v: Variables, stampedBetree: StampedBetree)
+    requires Init(v, stampedBetree)
+    ensures PivotBetree.Init(I(v), IStampedBetree(stampedBetree))
+  {
+  }
+
+//   lemma AllKeysInTotalDomain(key: Key)
+//     ensures key in TotalDomain().KeySet()
+//     ensures TotalDomain().Contains(key)
+//   {
+//     SmallestElementLte(Element(key));
+//   }
+
+//   lemma InternalGrowStepRefines(v: Variables, v': Variables, lbl: TransitionLabel, step: Step)
+//     requires Inv(v)
+//     requires NextStep(v, v', lbl, step)
+//     requires step.InternalGrowStep?
+//     ensures v'.WF()
+//     ensures PagedBetree.NextStep(I(v), I(v'), ILbl(lbl), IStep(step))
+//   {
+//     INodeWF(v.root);
+//     INodeWF(v'.root);
+//     assert I(v').root.children.mapp.Keys == AllKeys();  // trigger
+//     forall key:Key | AnyKey(key)
+//       ensures I(v').root.Child(key)
+//           == PagedBetree.ConstantChildMap(I(v).root).mapp[key] {
+//       AllKeysInTotalDomain(key);
+//       ChildCommutesWithI(v'.root, key);
+//     }
+//   }
+
+//   lemma SubstitutePreservesWF(path: Path, target': BetreeNode)
+//     requires path.Valid()
+//     requires path.ValidReplacement(target')
+//     ensures path.Substitute(target').WF()
+//   {}
+
+//   // Substitution followed by interpretation is the same as interpretation
+//   // followed by paged-level substitution.
+//   lemma SubstitutionRefines(path: Path, target': BetreeNode)
+//     requires path.Valid()
+//     requires path.ValidReplacement(target')
+//     ensures path.Substitute(target').WF()
+//     ensures IPath(path).Valid()
+//     ensures INode(target').WF();
+//     ensures INode(path.Substitute(target')) == IPath(path).Substitute(INode(target'));
+//     decreases path.depth;
+//   {
+//     IPathValid(path);
+//     SubstitutePreservesWF(path, target');
+//     IPathValid(path);
+//     INodeWF(target');
+//     if path.depth==0 {
+//       assert INode(path.Substitute(target')) == IPath(path).Substitute(INode(target'));
+//     } else {
+//       SubstitutionRefines(path.Subpath(), target');
+//       forall key ensures
+//         IChildren(path.Substitute(target')).mapp[key]
+//         == IPath(path).ReplacedChildren(INode(target')).mapp[key] 
+//       {
+//         if key in path.node.KeySet() {
+//           if Route(path.node.pivotTable, path.key) == Route(path.node.pivotTable, key) {
+//             var replacedChild := IPath(path).Subpath().Substitute(INode(target'));
+//             assert replacedChild == IPath(path).ReplacedChildren(INode(target')).mapp[key] by {
+//               IPath(path).reveal_ReplacedChildren();  // protected in by clause to avoid timeout
+//             }
+//             SubpathCommutesWithIPath(path);
+//           } else {
+//             assert IPath(path).node.Child(key) == IPath(path).ReplacedChildren(INode(target')).mapp[key] by {
+//               IPath(path).reveal_ReplacedChildren();  // protected in by clause to avoid timeout
+//             }
+//             ChildCommutesWithI(path.node, key);
+//           }
+//         } else {
+//           assert PagedBetree.Nil == INode(path.node).Child(key);  // trigger
+//           assert IPath(path).node.Child(key) == IPath(path).ReplacedChildren(INode(target')).mapp[key] by {
+//             IPath(path).reveal_ReplacedChildren();  // protected in by clause to avoid timeout
+//           }
+//         }
+//       }
+//       assert INode(path.Substitute(target')) == IPath(path).Substitute(INode(target'));  // trigger
+//     }
+//   }
+
+//   lemma TargetCommutesWithI(path: Path) 
+//     requires path.Valid()
+//     ensures IPath(path).Valid()  // prereq
+//     ensures IPath(path).Target() == INode(path.Target())
+//     decreases path.depth
+//   {
+//     IPathValid(path);
+//     if 0 < path.depth {
+//       TargetCommutesWithI(path.Subpath());
+//       SubpathCommutesWithIPath(path);
+//       assert IPath(path).Target() == INode(path.Target());
+//     }
+//   }
+
+//   lemma SplitCommutesWithILeft(step: Step, key: Key)
+//     requires step.InternalSplitStep?
+//     requires step.WF()
+//     requires key in SplitLeftKeys(step)
+//     requires key in step.path.Target().KeySet()
+//     ensures
+//       var leftKeys := SplitLeftKeys(step);
+//       var t := step.path.Target();
+//       INode(t).Split(leftKeys, SplitChildKeys(step) - leftKeys).Child(key) == IChildren(t.SplitParent(step.request)).mapp[key];
+//   {
+//     var t := step.path.Target();
+//     var childDom := t.DomainRoutedToChild(step.request.childIdx);
+//     var leftDom := Domain(childDom.start, Element(step.SplitKey()));
+//     var leftKeys := SplitLeftKeys(step);
+//     var rightKeys := SplitChildKeys(step) - SplitLeftKeys(step);
+
+//     assert leftDom.KeySet() == leftKeys by {
+//       Keyspace.reveal_IsStrictlySorted();
+//       Keyspace.lteTransitiveForall();
+//     }
+//     if step.request.SplitLeaf? {
+//       assert INode(t.Child(key)).FilterBuffersAndChildren(leftDom.KeySet()).children == INode(t.Child(key).SplitLeaf(step.request.splitKey).0).children;  // trigger seq extensionality
+//     } else {
+//       assert INode(t.Child(key)).FilterBuffersAndChildren(leftDom.KeySet()).children == INode(t.Child(key).SplitIndex(step.request.childPivotIdx).0).children;  // trigger seq extensionality
+//     }
+//   }
+
+//   lemma SplitCommutesWithIRight(step: Step, key: Key)
+//     requires step.InternalSplitStep?
+//     requires step.WF()
+//     requires key in SplitChildKeys(step) - SplitLeftKeys(step)
+//     requires key in step.path.Target().KeySet()
+//     ensures
+//       var leftKeys := SplitLeftKeys(step);
+//       var t := step.path.Target();
+//       INode(t).Split(leftKeys, SplitChildKeys(step) - leftKeys).Child(key) == IChildren(t.SplitParent(step.request)).mapp[key];
+//   {
+//     var t := step.path.Target();
+//     var childDom := t.DomainRoutedToChild(step.request.childIdx);
+//     var rightDom := Domain(Element(step.SplitKey()), childDom.end);
+//     var leftKeys := SplitLeftKeys(step);
+//     var rightKeys := SplitChildKeys(step) - leftKeys;
+
+//     assert rightDom.KeySet() == rightKeys by {
+//       Keyspace.reveal_IsStrictlySorted();
+//       Keyspace.lteTransitiveForall();
+//     }
+//     if step.request.SplitLeaf? {
+//       assert INode(t.Child(key)).FilterBuffersAndChildren(rightDom.KeySet()).children == INode(t.Child(key).SplitLeaf(step.request.splitKey).1).children;  // trigger seq extensionality
+//     } else {
+//       assert INode(t.Child(key)).FilterBuffersAndChildren(rightDom.KeySet()).children == INode(t.Child(key).SplitIndex(step.request.childPivotIdx).1).children;  // trigger seq extensionality
+//     }
+//   }
+
+//   lemma SplitCommutesWithI(step: Step) 
+//     requires step.InternalSplitStep?
+//     requires step.WF()
+//     ensures INode(step.path.Target()).Split(SplitLeftKeys(step), SplitChildKeys(step) - SplitLeftKeys(step)) == INode(step.path.Target().SplitParent(step.request))
+//   {
+//     var leftKeys := SplitLeftKeys(step);
+//     var rightKeys := SplitChildKeys(step) - SplitLeftKeys(step);
+//     var t := step.path.Target();
+
+//     forall key | AnyKey(key)
+//     ensures INode(t).Split(leftKeys, rightKeys).Child(key)
+//       == IChildren(t.SplitParent(step.request)).mapp[key] 
+//     {
+//       if key in t.KeySet() {
+//         if key in leftKeys {
+//           SplitCommutesWithILeft(step, key);
+//         } else if key in rightKeys {
+//           SplitCommutesWithIRight(step, key);
+//         }
+//       }
+//     }
+//     assert PagedBetree.BetreeNode(t.buffers, IChildren(t)).Split(leftKeys, rightKeys).children.mapp.Keys
+//         == IChildren(t.SplitParent(step.request)).mapp.Keys;  // triggers extensionality
+//   }
+
+//   lemma InternalSplitStepRefines(v: Variables, v': Variables, lbl: TransitionLabel, step: Step)
+//     requires Inv(v)
+//     requires NextStep(v, v', lbl, step)
+//     requires step.InternalSplitStep?
+//     ensures v'.WF()
+//     ensures PagedBetree.NextStep(I(v), I(v'), ILbl(lbl), IStep(step))
+//   {
+//     INodeWF(v.root);
+//     INodeWF(step.path.Target());
+//     InvNext(v, v', lbl); //assert v'.WF();
+//     INodeWF(v'.root);
+//     IPathValid(step.path); //assert IPath(step.path).Valid();
+//     TargetCommutesWithI(step.path);
+//     SplitCommutesWithI(step);
+//     SubstitutionRefines(step.path, step.path.Target().SplitParent(step.request));
+//   }
+
+//   lemma PromoteCommutesWithI(node: BetreeNode, domain: Domain)  
+//     requires node.WF()
+//     requires domain.WF()
+//     requires domain.Domain?
+//     ensures INode(node.Promote(domain)) == INode(node).Promote()
+//   {
+//     assert INode(node.Promote(domain)) == INode(node).Promote();  // trigger
+//   }
+
+//   lemma PushBufferCommutesWithI(node: BetreeNode, buffers: BufferStack) 
+//     requires node.WF()
+//     requires node.BetreeNode?
+//     ensures INode(node.PushBufferStack(buffers)) == INode(node).PushBufferStack(buffers)
+//   {
+//     assert INode(node.PushBufferStack(buffers)).buffers == INode(node).PushBufferStack(buffers).buffers;  // trigger
+//   }
+
+//   // todo: this is duplicated in Journal/LinkedJournalRefinement
+//   lemma CommuteTransitivity<L,H>(I: L->H, f: L->L, F: H->H, g: L->L, G: H->H)
+//     requires forall x :: I(f(x))==F(I(x))
+//     requires forall x :: I(g(x))==G(I(x))
+//     ensures forall x :: I(g(f(x)))==G(F(I(x)))
+//   {
+//     // See Tony's phone cam picture of the proof that we wrote on the whiteboard
+//     // but which dafny doesn't need; eyeroll
+//   }
+  
+//   // TODO(tony): a much easier proof would be to condition on the nullity of node to factor out Promote()
+//   lemma PromoteComposedWithPushCommutes(node: BetreeNode, promoteDomain: Domain, buffers: BufferStack)  
+//     requires node.WF()
+//     requires promoteDomain.WF()
+//     requires promoteDomain.Domain?
+//     ensures INode(node.Promote(promoteDomain).PushBufferStack(buffers)) 
+//         == INode(node).Promote().PushBufferStack(buffers);
+//   {
+//     EmptyDomain.reveal_SaneKeys();
+//     var dummy := EmptyRoot(promoteDomain);  // using promoteDomain as placeholder. It doesn't matter what domain is used
+//     var idummy := PagedBetree.EmptyRoot();
+//     var i := (n: BetreeNode) => if n.WF() && n.BetreeNode? then INode(n) else idummy;
+//     var f := (n: BetreeNode) => if n.WF() then n.Promote(promoteDomain) else dummy;
+//     var g := (n: BetreeNode) => if n.WF() && n.BetreeNode? then n.PushBufferStack(buffers) else dummy.PushBufferStack(buffers);  // this is a clever trick to use dummy.PushBufferStack(buffers), so that the commutativity aligns
+//     var F := (pn: PagedBetree.BetreeNode) => if pn.WF() then pn.Promote() else idummy;
+//     var G := (pn: PagedBetree.BetreeNode) => if pn.WF() && pn.BetreeNode? then pn.PushBufferStack(buffers) else idummy;
+
+//     forall n ensures i(f(n)) == F(i(n))
+//     {
+//       if n.WF() {
+//         PromoteCommutesWithI(n, promoteDomain);
+//       } else {
+//         PushBufferCommutesWithI(EmptyRoot(promoteDomain), buffers); 
+//         assert IChildren(EmptyRoot(promoteDomain)) == PagedBetree.ConstantChildMap(PagedBetree.Nil);  // trigger
+//       }
+//     }
+//     assert INode(f(node)) == F(INode(node));  // trigger
+//     forall n ensures i(g(n)) == G(i(n))
+//     {
+//       if n.WF() && n.BetreeNode? {
+//         calc {
+//           INode(n.PushBufferStack(buffers));
+//           { PushBufferCommutesWithI(n, buffers); }
+//           INode(n).PushBufferStack(buffers);
+//         }
+//       } else {
+//         PushBufferCommutesWithI(EmptyRoot(promoteDomain), buffers);
+//         assert IChildren(EmptyRoot(promoteDomain)) == PagedBetree.ConstantChildMap(PagedBetree.Nil);
+//       }
+//     }
+//     CommuteTransitivity(i, f, F, g, G);
+//   }
+
+//   lemma FlushCommutesWithI(step: Step) 
+//     requires step.InternalFlushStep?
+//     requires step.WF()
+//     ensures INode(step.path.Target()).Flush(IStep(step).downKeys) == INode(step.path.Target().Flush(step.childIdx))
+//   {
+//     var t := step.path.Target();
+//     var istep := IStep(step);
+//     forall k | AnyKey(k) 
+//     ensures INode(t.Flush(step.childIdx)).Child(k) == INode(t).Flush(istep.downKeys).Child(k)
+//     {
+//       if k in istep.downKeys {
+//         assert t.KeyInDomain(k) by {
+//           Keyspace.reveal_IsSorted();
+//           Keyspace.lteTransitiveForall();
+//         }
+//         ChildCommutesWithI(t.Flush(step.childIdx), k);
+//         var newBuffers := t.buffers.ApplyFilter(t.DomainRoutedToChild(step.childIdx).KeySet());
+//         PromoteComposedWithPushCommutes(t.children[step.childIdx], t.DomainRoutedToChild(step.childIdx), newBuffers);
+//       }
+//     }
+//     assert INode(step.path.Target()).Flush(IStep(step).downKeys) == INode(step.path.Target().Flush(step.childIdx));  // trigger
+//   }
+
+//   lemma InternalFlushStepRefines(v: Variables, v': Variables, lbl: TransitionLabel, step: Step)
+//     requires Inv(v)
+//     requires NextStep(v, v', lbl, step)
+//     requires step.InternalFlushStep?
+//     ensures v'.WF()
+//     ensures PagedBetree.NextStep(I(v), I(v'), ILbl(lbl), IStep(step))
+//   {
+//     INodeWF(v.root);
+//     INodeWF(step.path.Target());
+//     InvNext(v, v', lbl); //assert v'.WF();
+//     INodeWF(v'.root);
+//     IPathValid(step.path); //assert IPath(step.path).Valid();
+//     TargetCommutesWithI(step.path);
+//     FlushCommutesWithI(step);
+//     SubstitutionRefines(step.path, step.path.Target().Flush(step.childIdx));
+//   }
+
+//   predicate EquivalentBufferCompaction(node: BetreeNode, other: BetreeNode)
+//   {
+//     && node.WF()
+//     && other.WF()
+//     && node.BetreeNode?
+//     && other.BetreeNode?
+//     && node.buffers.Equivalent(other.buffers)
+//     && node.pivotTable == other.pivotTable
+//     && node.children == other.children
+//   }
+
+//   lemma BufferCompactionRefines(node: BetreeNode, other: BetreeNode)
+//     requires EquivalentBufferCompaction(node, other)
+//     ensures PagedBetreeRefinement.EquivalentBufferCompaction(INode(node), INode(other))
+//   {}
+
+//   lemma InternalCompactStepRefines(v: Variables, v': Variables, lbl: TransitionLabel, step: Step)
+//     requires Inv(v)
+//     requires NextStep(v, v', lbl, step)
+//     requires step.InternalCompactStep?
+//     ensures v'.WF()
+//     ensures PagedBetree.NextStep(I(v), I(v'), ILbl(lbl), IStep(step))
+//   {
+//     INodeWF(v.root);
+//     INodeWF(step.path.Target());
+//     InvNext(v, v', lbl); //assert v'.WF();
+//     INodeWF(v'.root);
+//     IPathValid(step.path); //assert IPath(step.path).Valid();
+//     var compactedNode := CompactedNode(step.path.Target(), step.compactedBuffers);
+//     SubstitutionRefines(step.path, compactedNode);
+//     BufferCompactionRefines(step.path.Target(), compactedNode);
+//     TargetCommutesWithI(step.path);
+//   }
+
+  // lemma FreezeAsRefines(v: Variables, v': Variables, lbl: TransitionLabel, step: Step)
+  //   requires Inv(v)
+  //   requires NextStep(v, v', lbl, step)
+  //   requires step.FreezeAsStep?
+  //   ensures v'.WF()
+  //   ensures PivotBetree.NextStep(I(v), I(v'), ILbl(lbl), IStep(step))
+  // {
+  //   assert INode(PushMemtable(v.root, v.memtable).value) == PivotBetree.PushMemtable(INode(v.root), v.memtable).value;
+  // }
+
+  // lemma InternalFlushMemtableStepRefines(v: Variables, v': Variables, lbl: TransitionLabel, step: Step)
+  //   requires Inv(v)
+  //   requires NextStep(v, v', lbl, step)
+  //   requires step.InternalFlushMemtableStep?
+  //   ensures v'.WF()
+  //   ensures PivotBetree.NextStep(I(v), I(v'), ILbl(lbl), IStep(step))
+  // {
+  //   assert INode(PushMemtable(v.root, v.memtable).value) == PivotBetree.PushMemtable(INode(v.root), v.memtable).value;
+  // }
+
+  // lemma NextRefines(v: Variables, v': Variables, lbl: TransitionLabel)
+  //   requires Inv(v)
+  //   requires Next(v, v', lbl)
+  //   ensures v'.WF()
+  //   ensures PivotBetree.Next(I(v), I(v'), ILbl(lbl))
+  // {
+  //   InvNext(v, v', lbl);
+  //   var step: Step :| NextStep(v, v', lbl, step);
+  //   match step {
+  //     case QueryStep(receipt) => {
+  //       ValidReceiptRefines(step.receipt);
+  //       assert PivotBetree.NextStep(I(v), I(v'), ILbl(lbl), IStep(step)); // trigger
+  //     }
+  //     case PutStep() => {
+  //       assert PivotBetree.NextStep(I(v), I(v'), ILbl(lbl), IStep(step));
+  //     }
+  //     case QueryEndLsnStep() => {
+  //       assert PivotBetree.NextStep(I(v), I(v'), ILbl(lbl), IStep(step));
+  //     }
+  //     case FreezeAsStep() => {
+  //       INodeWF(v.root);
+  //       FreezeAsRefines(v, v', lbl, step);
+  //       assert PivotBetree.NextStep(I(v), I(v'), ILbl(lbl), IStep(step)); 
+  //     }
+  //     case InternalGrowStep() => {
+  //       InternalGrowStepRefines(v, v', lbl, step);
+  //     }
+  //     case InternalSplitStep(_, _) => {
+  //       InternalSplitStepRefines(v, v', lbl, step);
+  //       assert PivotBetree.NextStep(I(v), I(v'), ILbl(lbl), IStep(step));
+  //     }
+  //     case InternalFlushStep(_, _) => {
+  //       InternalFlushStepRefines(v, v', lbl, step);
+  //       assert PivotBetree.NextStep(I(v), I(v'), ILbl(lbl), IStep(step));
+  //     }
+  //     case InternalFlushMemtableStep() => {
+  //       InternalFlushMemtableStepRefines(v, v', lbl, step);
+  //       assert PivotBetree.NextStep(I(v), I(v'), ILbl(lbl), IStep(step));
+  //     }
+  //     case InternalCompactStep(_, _) => {
+  //       InternalCompactStepRefines(v, v', lbl, step);
+  //       assert PivotBetree.NextStep(I(v), I(v'), ILbl(lbl), IStep(step));
+  //     }
+  //     case InternalNoOpStep() => 
+  //        assert PivotBetree.NextStep(I(v), I(v'), ILbl(lbl), IStep(step));
+  //   }
+  // }
+}
